Fixed some bugs on the MSI protocol

src/Ex/MsiSv.v
@@ -2,7 +2,7 @@ Require Import Bool Vector List String Peano_dec.
 Require Import Common FMap HVector ListSupport Syntax Semantics StepT.
 Require Import Topology RqRs.
 
-Require Import Msi.
+Require Import Spec SpecSv Msi.
 
 Set Implicit Arguments.
 
@@ -12,493 +12,398 @@ Open Scope fmap.
 
 Section System.
 
-  Definition erq1 := 0.
-  Definition ers1 := 1.
-  Definition erq2 := 2.
-  Definition ers2 := 3.
+  Definition erq1 := erq 0.
+  Definition ers1 := ers 0.
+  Definition erq2 := erq 1.
+  Definition ers2 := ers 1.
 
-  Section Spec.
-
-    Definition specIdx := 0.
-
-    Definition SpecOStateIfc: OStateIfc :=
-      {| ost_sz := 1;
-         ost_ty := [nat:Type]%vector |}.
-    Definition specValueIdx: Fin.t 1 := Fin.F1.
+  Definition ec1 := 4.
+  Definition ce1 := 5.
+  Definition ec2 := 6.
+  Definition ce2 := 7.
+  Definition c1pRq := 8.
+  Definition c1pRs := 9.
+  Definition pc1 := 10.
+  Definition c2pRq := 11.
+  Definition c2pRs := 12.
+  Definition pc2 := 13.
     
-    Section PerChn.
-      Variable ridxOfs: nat.
-      Variables (erq ers: nat).
+  Definition parentIdx := 0.
+  Definition child1Idx := 1.
+  Definition child2Idx := 2.
 
-      Definition specNumOfRules := 3.
-      
-      Definition specGetRq: Rule SpecOStateIfc :=
-        {| rule_idx := specNumOfRules * ridxOfs + 0;
-           rule_msg_ids := [msiGetRq];
-           rule_msgs_from := fun _ => [erq];
-           rule_precond := ⊤oprec;
-           rule_trs :=
-             fun (ost: OState SpecOStateIfc) orq mins =>
-               (ost, orq,
-                [(ers, {| msg_id := msiGetRs;
-                          msg_value := VNat (ost#[specValueIdx])
-                       |})])
-        |}.
+  Definition implValueIdx: Fin.t 2 := Fin.F1.
+  Definition implStatusIdx: Fin.t 2 := Fin.FS Fin.F1.
+  
+  Definition ImplOStateIfc: OStateIfc :=
+    {| ost_sz := 2;
+       ost_ty := [nat:Type; nat:Type]%vector |}.
+  Definition implInit: OStates :=
+    [parentIdx <- {| ost_ifc := ImplOStateIfc;
+                     ost_st := (0, (msiS, tt)) |}]
+    +[child1Idx <- {| ost_ifc := ImplOStateIfc;
+                      ost_st := (0, (msiS, tt)) |}]
+    +[child2Idx <- {| ost_ifc := ImplOStateIfc;
+                      ost_st := (0, (msiS, tt)) |}].
 
-      Definition specSetRq: Rule SpecOStateIfc :=
-        {| rule_idx := specNumOfRules * ridxOfs + 1;
-           rule_msg_ids := [msiSetRq];
-           rule_msgs_from := fun _ => [erq];
-           rule_precond := ⊤oprec;
-           rule_trs :=
-             fun (ost: OState SpecOStateIfc) orq mins =>
-               ((hd_error mins) >>=[ost]
-                  (fun idm =>
-                     match msg_value (valOf idm) with
-                     | VNat n => ost+#[specValueIdx <- n]
-                     | _ => ost
-                     end),
-                orq,
-                [(ers, {| msg_id := msiSetRs;
-                          msg_value := VUnit |})])
-        |}.
+  Section Child.
+    Variable (coidx: IdxT).
+    Variables (ec ce cpRq cpRs pc: IdxT).
 
-      Definition specEvictRq: Rule SpecOStateIfc :=
-        {| rule_idx := specNumOfRules * ridxOfs + 2;
-           rule_msg_ids := [msiEvictRq];
-           rule_msgs_from := fun _ => [erq];
-           rule_precond := ⊤oprec;
-           rule_trs :=
-             fun (ost: OState SpecOStateIfc) orq mins =>
-               (ost, orq,
-                [(ers, {| msg_id := msiEvictRs;
-                          msg_value := VUnit |})])
-        |}.
-      
-    End PerChn.
-
-    Definition specInit: OStates :=
-      [specIdx <- {| ost_ifc := SpecOStateIfc;
-                     ost_st := hvcons 0 hvnil (* (0, tt) *) |}].
-
-    Definition specObj: Object :=
-      {| obj_idx := specIdx;
-         obj_ifc := SpecOStateIfc;
-         obj_rules := 
-           [specGetRq 0 erq1 ers1;
-              specSetRq 0 erq1 ers1;
-              specEvictRq 0 erq1 ers1;
-              specGetRq 1 erq2 ers2;
-              specSetRq 1 erq2 ers2;
-              specEvictRq 1 erq2 ers2];
-         obj_rules_valid := ltac:(inds_valid_tac)
-      |}.
-    
-    Definition spec: System :=
-      {| sys_objs := [specObj];
-         sys_oinds_valid := ltac:(inds_valid_tac);
-         sys_minds := nil;
-         sys_merqs := [erq1; erq2];
-         sys_merss := [ers1; ers2];
-         sys_msg_inds_valid := ltac:(inds_valid_tac);
-         sys_oss_inits := specInit;
-         sys_orqs_inits := []
+    Definition childGetRqImm: Rule ImplOStateIfc :=
+      {| rule_idx := 0;
+         rule_msg_ids := [getRq];
+         rule_msgs_from := fun _ => [ec];
+         rule_precond :=
+           fun (ost: OState ImplOStateIfc) orq mins =>
+             LockFree orq O /\ ost#[implStatusIdx] >= msiS;
+         rule_trs :=
+           fun (ost: OState ImplOStateIfc) orq mins =>
+             (ost, orq,
+              [(ce, {| msg_id := getRs;
+                       msg_value := VNat (ost#[implValueIdx])
+                    |})])
       |}.
 
-  End Spec.
+    Definition childGetRqS: Rule ImplOStateIfc :=
+      {| rule_idx := 1;
+         rule_msg_ids := [getRq];
+         rule_msgs_from := fun _ => [ec];
+         rule_precond :=
+           fun (ost: OState ImplOStateIfc) orq mins =>
+             LockFree orq O /\ ost#[implStatusIdx] = msiI;
+         rule_trs :=
+           fun (ost: OState ImplOStateIfc) orq mins =>
+             ((hd_error mins) >>=[(ost, orq, nil)]
+               (fun idm =>
+                  (ost,
+                   addRq orq O upRq (valOf idm) [pc] ce,
+                   [(cpRq, {| msg_id := msiRqS;
+                              msg_value := VUnit |})])))
+      |}.
 
-  Section Impl.
+    Definition childGetRsS: Rule ImplOStateIfc :=
+      {| rule_idx := 2;
+         rule_msg_ids := [msiRsS];
+         rule_msgs_from := fun _ => [pc];
+         rule_precond := ⊤oprec;
+         rule_trs :=
+           fun (ost: OState ImplOStateIfc) orq mins =>
+             ((hd_error mins) >>=[(ost, orq, nil)]
+               (fun idm =>
+                  match msg_value (valOf idm) with
+                  | VNat n =>
+                    (ost +#[implValueIdx <- n] +#[implStatusIdx <- msiS],
+                     removeRq orq O upRq,
+                     [(ce, {| msg_id := getRs;
+                              msg_value := VNat n |})])
+                  | _ => (ost, orq, nil) (** TODO: how to efficiently handle this case? *)
+                  end))
+      |}.
 
-    Definition ec1 := 4.
-    Definition ce1 := 5.
-    Definition ec2 := 6.
-    Definition ce2 := 7.
-    Definition c1pRq := 8.
-    Definition c1pRs := 9.
-    Definition pc1 := 10.
-    Definition c2pRq := 11.
-    Definition c2pRs := 12.
-    Definition pc2 := 13.
+    Definition childDownRqS: Rule ImplOStateIfc :=
+      {| rule_idx := 3;
+         rule_msg_ids := [msiDownRqS];
+         rule_msgs_from := fun _ => [pc];
+         rule_precond :=
+           fun (ost: OState ImplOStateIfc) orq mins =>
+             HalfLockFree orq O;
+         rule_trs :=
+           fun (ost: OState ImplOStateIfc) orq mins =>
+             (ost+#[implStatusIdx <- msiS],
+              orq,
+              [(cpRs, {| msg_id := msiDownRsS;
+                         msg_value := VUnit |})])
+      |}.
+
+    Definition childSetRqImm: Rule ImplOStateIfc :=
+      {| rule_idx := 4;
+         rule_msg_ids := [setRq];
+         rule_msgs_from := fun _ => [ec];
+         rule_precond :=
+           fun (ost: OState ImplOStateIfc) orq mins =>
+             LockFree orq O /\ ost#[implStatusIdx] = msiM;
+         rule_trs :=
+           fun (ost: OState ImplOStateIfc) orq mins =>
+             ((hd_error mins) >>=[(ost, orq, nil)]
+               (fun idm =>
+                  match msg_value (valOf idm) with
+                  | VNat n =>
+                    (ost +#[implValueIdx <- n] +#[implStatusIdx <- msiM],
+                     orq,
+                     [(ce, {| msg_id := setRs;
+                              msg_value := VUnit |})])
+                  | _ => (ost, orq, nil)
+                  end))
+      |}.
     
-    Definition parentIdx := 0.
-    Definition child1Idx := 1.
-    Definition child2Idx := 2.
+    Definition childSetRqM: Rule ImplOStateIfc :=
+      {| rule_idx := 5;
+         rule_msg_ids := [setRq];
+         rule_msgs_from := fun _ => [ec];
+         rule_precond :=
+           fun (ost: OState ImplOStateIfc) orq mins =>
+             LockFree orq O /\ ost#[implStatusIdx] <> msiM;
+         rule_trs :=
+           fun (ost: OState ImplOStateIfc) orq mins =>
+             ((hd_error mins) >>=[(ost, orq, nil)]
+               (fun idm =>
+                  (ost,
+                   addRq orq O upRq (valOf idm) [pc] ce,
+                   [(cpRq, {| msg_id := msiRqM;
+                              msg_value := VUnit |})])))
+      |}.
 
-    Definition implValueIdx: Fin.t 2 := Fin.F1.
-    Definition implStatusIdx: Fin.t 2 := Fin.FS Fin.F1.
+    Definition childSetRsM: Rule ImplOStateIfc :=
+      {| rule_idx := 6;
+         rule_msg_ids := [msiRsM];
+         rule_msgs_from := fun _ => [pc];
+         rule_precond := ⊤oprec;
+         rule_trs :=
+           fun (ost: OState ImplOStateIfc) orq mins =>
+             (Syntax.getRq orq O upRq) >>=[(ost, orq, nil)]
+               (fun rqinfo =>
+                  match msg_value (rqi_msg rqinfo) with
+                  | VNat n =>
+                    (ost +#[implValueIdx <- n] +#[implStatusIdx <- msiM],
+                     removeRq orq O upRq,
+                     (ce,
+                      {| msg_id := setRs;
+                         msg_value := VNat n |}) :: nil)
+                  | _ => (ost, orq, nil)
+                  end)
+      |}.
+
+    Definition childDownRqM: Rule ImplOStateIfc :=
+      {| rule_idx := 7;
+         rule_msg_ids := [msiDownRqM];
+         rule_msgs_from := fun _ => [pc];
+         rule_precond :=
+           fun (ost: OState ImplOStateIfc) orq mins =>
+             HalfLockFree orq O;
+         rule_trs :=
+           fun (ost: OState ImplOStateIfc) orq mins =>
+             (ost +#[implStatusIdx <- msiI],
+              orq,
+              [(cpRs, {| msg_id := msiDownRsS;
+                         msg_value := VNat (ost#[implValueIdx]) |})])
+      |}.
+
+    Definition childEvictRqI: Rule ImplOStateIfc :=
+      {| rule_idx := 8;
+         rule_msg_ids := nil;
+         rule_msgs_from := fun _ => nil;
+         rule_precond :=
+           fun (ost: OState ImplOStateIfc) orq mins =>
+             LockFree orq O /\ ost#[implStatusIdx] <> msiI;
+         rule_trs :=
+           fun (ost: OState ImplOStateIfc) orq mins =>
+             ((hd_error mins) >>=[(ost, orq, nil)]
+               (fun idm =>
+                  (ost,
+                   addRq orq O upRq (valOf idm) [pc] ce,
+                   [(cpRq, {| msg_id := msiRqI;
+                              msg_value := VNat (ost#[implValueIdx]) |})])))
+      |}.
+
+    Definition childEvictRsI: Rule ImplOStateIfc :=
+      {| rule_idx := 9;
+         rule_msg_ids := [msiRsI];
+         rule_msgs_from := fun _ => [pc];
+         rule_precond := ⊤oprec;
+         rule_trs :=
+           fun (ost: OState ImplOStateIfc) orq mins =>
+             ((hd_error mins) >>=[(ost, orq, nil)]
+               (fun idm =>
+                  (ost +#[implStatusIdx <- msiI],
+                   removeRq orq O upRq,
+                   nil)))
+      |}.
+      
+    Definition child: Object :=
+      {| obj_idx := coidx;
+         obj_ifc := ImplOStateIfc;
+         obj_rules :=
+           [childGetRqImm; childGetRqS; childGetRsS; childDownRqS;
+              childSetRqImm; childSetRqM; childSetRsM; childDownRqM;
+                childEvictRqI; childEvictRsI];
+         obj_rules_valid := ltac:(inds_valid_tac) |}.
+
+  End Child.
     
-    Definition ImplOStateIfc: OStateIfc :=
-      {| ost_sz := 2;
-         ost_ty := [nat:Type; nat:Type]%vector |}.
-    Definition implInit: OStates :=
-      [parentIdx <- {| ost_ifc := ImplOStateIfc;
-                       ost_st := (0, (msiS, tt)) |}]
-      +[child1Idx <- {| ost_ifc := ImplOStateIfc;
-                        ost_st := (0, (msiS, tt)) |}]
-      +[child2Idx <- {| ost_ifc := ImplOStateIfc;
-                        ost_st := (0, (msiS, tt)) |}].
+  Section Parent.
 
-    Section Child.
-      Variable (coidx: IdxT).
-      Variables (ec ce cpRq cpRs pc: IdxT).
+    Section Rules.
+      Variable (ridxOfs: IdxT).
+      Variables (cpRq pc cpRs' pc': IdxT).
 
-      Definition childGetRqImm: Rule ImplOStateIfc :=
-        {| rule_idx := 0;
-           rule_msg_ids := [msiGetRq];
-           rule_msgs_from := fun _ => [ec];
+      Definition parentNumOfRules := 7.
+
+      Definition parentGetRqImm: Rule ImplOStateIfc :=
+        {| rule_idx := parentNumOfRules * ridxOfs + 0;
+           rule_msg_ids := [msiRqS];
+           rule_msgs_from := fun _ => [cpRq];
            rule_precond :=
              fun (ost: OState ImplOStateIfc) orq mins =>
                LockFree orq O /\ ost#[implStatusIdx] >= msiS;
            rule_trs :=
              fun (ost: OState ImplOStateIfc) orq mins =>
                (ost, orq,
-                [(ce, {| msg_id := msiGetRs;
-                         msg_value := VNat (ost#[implValueIdx])
-                      |})])
+                [(pc, {| msg_id := msiRsS;
+                         msg_value := VNat (ost#[implValueIdx]) |})])
         |}.
 
-      Definition childGetRqS: Rule ImplOStateIfc :=
-        {| rule_idx := 1;
-           rule_msg_ids := [msiGetRq];
-           rule_msgs_from := fun _ => [ec];
+      Definition parentGetDownRqS: Rule ImplOStateIfc :=
+        {| rule_idx := parentNumOfRules * ridxOfs + 1;
+           rule_msg_ids := [msiRqS];
+           rule_msgs_from := fun _ => [cpRq];
            rule_precond :=
              fun (ost: OState ImplOStateIfc) orq mins =>
                LockFree orq O /\ ost#[implStatusIdx] = msiI;
            rule_trs :=
              fun (ost: OState ImplOStateIfc) orq mins =>
                ((hd_error mins) >>=[(ost, orq, nil)]
-                  (fun idm =>
-                     (ost,
-                      addRq orq O upRq (valOf idm) [pc] ce,
-                      [(cpRq, {| msg_id := msiRqS;
-                                 msg_value := VUnit |})])))
+                 (fun idm =>
+                    (ost,
+                     addRq orq O downRq (valOf idm) [cpRs'] pc,
+                     [(pc', {| msg_id := msiDownRqS;
+                               msg_value := VNat (ost#[implValueIdx]) |})])))
         |}.
 
-      Definition childGetRsS: Rule ImplOStateIfc :=
-        {| rule_idx := 2;
-           rule_msg_ids := [msiRsS];
-           rule_msgs_from := fun _ => [pc];
+      Definition parentGetDownRsS: Rule ImplOStateIfc :=
+        {| rule_idx := parentNumOfRules * ridxOfs + 2;
+           rule_msg_ids := [msiDownRsS];
+           rule_msgs_from := fun _ => [cpRs'];
            rule_precond := ⊤oprec;
            rule_trs :=
              fun (ost: OState ImplOStateIfc) orq mins =>
                ((hd_error mins) >>=[(ost, orq, nil)]
-                  (fun idm =>
-                     match msg_value (valOf idm) with
-                     | VNat n =>
-                       (ost +#[implValueIdx <- n] +#[implStatusIdx <- msiS],
-                        removeRq orq O upRq,
-                        [(ce, {| msg_id := msiGetRs;
-                                 msg_value := VNat n |})])
-                     | _ => (ost, orq, nil) (** TODO: how to efficiently handle this case? *)
-                     end))
+                 (fun idm =>
+                    match msg_value (valOf idm) with
+                    | VNat n =>
+                      (ost +#[implValueIdx <- n] +#[implStatusIdx <-msiS],
+                       removeRq orq O downRq,
+                       [(pc, {| msg_id := msiRsS;
+                                msg_value := VNat n |})])
+                    | _ => (ost, orq, nil)
+                    end))
         |}.
 
-      Definition childDownRqS: Rule ImplOStateIfc :=
-        {| rule_idx := 3;
-           rule_msg_ids := [msiDownRqS];
-           rule_msgs_from := fun _ => [pc];
-           rule_precond :=
-             fun (ost: OState ImplOStateIfc) orq mins =>
-               HalfLockFree orq O;
-           rule_trs :=
-             fun (ost: OState ImplOStateIfc) orq mins =>
-               (ost+#[implStatusIdx <- msiS],
-                orq,
-                [(cpRs, {| msg_id := msiDownRsS;
-                           msg_value := VUnit |})])
-        |}.
-
-      Definition childSetRqImm: Rule ImplOStateIfc :=
-        {| rule_idx := 4;
-           rule_msg_ids := [msiSetRq];
-           rule_msgs_from := fun _ => [ec];
+      Definition parentSetRqImm: Rule ImplOStateIfc :=
+        {| rule_idx := parentNumOfRules * ridxOfs + 3;
+           rule_msg_ids := [msiRqM];
+           rule_msgs_from := fun _ => [cpRq];
            rule_precond :=
              fun (ost: OState ImplOStateIfc) orq mins =>
                LockFree orq O /\ ost#[implStatusIdx] = msiM;
            rule_trs :=
              fun (ost: OState ImplOStateIfc) orq mins =>
-               ((hd_error mins) >>=[(ost, orq, nil)]
-                  (fun idm =>
-                     match msg_value (valOf idm) with
-                     | VNat n =>
-                       (ost +#[implValueIdx <- n] +#[implStatusIdx <- msiM],
-                        orq,
-                        [(ce, {| msg_id := msiSetRs;
-                                 msg_value := VUnit |})])
-                     | _ => (ost, orq, nil)
-                     end))
+               (ost +#[implStatusIdx <- msiI],
+                orq,
+                [(pc, {| msg_id := msiRsM;
+                         msg_value := VNat (ost#[implValueIdx]) |})])
         |}.
-    
-      Definition childSetRqM: Rule ImplOStateIfc :=
-        {| rule_idx := 5;
-           rule_msg_ids := [msiSetRq];
-           rule_msgs_from := fun _ => [ec];
+
+      Definition parentSetDownRqM: Rule ImplOStateIfc :=
+        {| rule_idx := parentNumOfRules * ridxOfs + 4;
+           rule_msg_ids := [msiRqM];
+           rule_msgs_from := fun _ => [cpRq];
            rule_precond :=
              fun (ost: OState ImplOStateIfc) orq mins =>
                LockFree orq O /\ ost#[implStatusIdx] <> msiM;
            rule_trs :=
              fun (ost: OState ImplOStateIfc) orq mins =>
                ((hd_error mins) >>=[(ost, orq, nil)]
-                  (fun idm =>
-                     (ost,
-                      addRq orq O upRq (valOf idm) [pc] ce,
-                      [(cpRq, {| msg_id := msiRqM;
-                                 msg_value := VUnit |})])))
-        |}.
-
-      Definition childSetRsM: Rule ImplOStateIfc :=
-        {| rule_idx := 6;
-           rule_msg_ids := [msiRsM];
-           rule_msgs_from := fun _ => [pc];
-           rule_precond := ⊤oprec;
-           rule_trs :=
-             fun (ost: OState ImplOStateIfc) orq mins =>
-               (getRq orq O upRq) >>=[(ost, orq, nil)]
-                 (fun rqinfo =>
-                    match msg_value (rqi_msg rqinfo) with
-                    | VNat n =>
-                      (ost +#[implValueIdx <- n] +#[implStatusIdx <- msiM],
-                       removeRq orq O upRq,
-                       (ce,
-                        {| msg_id := msiSetRs;
-                           msg_value := VNat n |}) :: nil)
-                    | _ => (ost, orq, nil)
-                    end)
-        |}.
-
-      Definition childDownRqM: Rule ImplOStateIfc :=
-        {| rule_idx := 7;
-           rule_msg_ids := [msiDownRqM];
-           rule_msgs_from := fun _ => [pc];
-           rule_precond :=
-             fun (ost: OState ImplOStateIfc) orq mins =>
-               HalfLockFree orq O;
-           rule_trs :=
-             fun (ost: OState ImplOStateIfc) orq mins =>
-               (ost +#[implStatusIdx <- msiI],
-                orq,
-                [(cpRs, {| msg_id := msiDownRsS;
-                           msg_value := VNat (ost#[implValueIdx]) |})])
-        |}.
-
-      Definition childEvictRqI: Rule ImplOStateIfc :=
-        {| rule_idx := 8;
-           rule_msg_ids := [msiEvictRq];
-           rule_msgs_from := fun _ => [ec];
-           rule_precond :=
-             fun (ost: OState ImplOStateIfc) orq mins =>
-               LockFree orq O /\ ost#[implStatusIdx] <> msiI;
-           rule_trs :=
-             fun (ost: OState ImplOStateIfc) orq mins =>
-               ((hd_error mins) >>=[(ost, orq, nil)]
-                  (fun idm =>
-                     (ost,
-                      addRq orq O upRq (valOf idm) [pc] ce,
-                      [(cpRq, {| msg_id := msiRqI;
-                                 msg_value := VNat (ost#[implValueIdx]) |})])))
-        |}.
-
-      Definition childEvictRsI: Rule ImplOStateIfc :=
-        {| rule_idx := 9;
-           rule_msg_ids := [msiRsI];
-           rule_msgs_from := fun _ => [pc];
-           rule_precond := ⊤oprec;
-           rule_trs :=
-             fun (ost: OState ImplOStateIfc) orq mins =>
-               ((hd_error mins) >>=[(ost, orq, nil)]
-                  (fun idm =>
-                     (ost +#[implStatusIdx <- msiI],
-                      removeRq orq O upRq,
-                      [(ce, {| msg_id := msiEvictRs;
+                 (fun idm =>
+                    (ost,
+                     addRq orq O downRq (valOf idm) [cpRs'] pc,
+                     [(pc', {| msg_id := msiDownRqM;
                                msg_value := VUnit |})])))
         |}.
-      
-      Definition child: Object :=
-        {| obj_idx := coidx;
-           obj_ifc := ImplOStateIfc;
-           obj_rules :=
-             [childGetRqImm; childGetRqS; childGetRsS; childDownRqS;
-                childSetRqImm; childSetRqM; childSetRsM; childDownRqM;
-                  childEvictRqI; childEvictRsI];
-           obj_rules_valid := ltac:(inds_valid_tac) |}.
-      
-    End Child.
 
-    Section Parent.
+      Definition parentSetDownRsM: Rule ImplOStateIfc :=
+        {| rule_idx := parentNumOfRules * ridxOfs + 5;
+           rule_msg_ids := [msiDownRsM];
+           rule_msgs_from := fun _ => [cpRs'];
+           rule_precond := ⊤oprec;
+           rule_trs :=
+             fun (ost: OState ImplOStateIfc) orq mins =>
+               ((hd_error mins) >>=[(ost, orq, nil)]
+                 (fun idm =>
+                    match msg_value (valOf idm) with
+                    | VNat n =>
+                      (ost +#[implStatusIdx <- msiI],
+                       removeRq orq O downRq,
+                       [(pc, {| msg_id := msiRsM;
+                                msg_value := VNat n |})])
+                    | _ => (ost, orq, nil)
+                    end))
+        |}.
 
-      Section Rules.
-        Variable (ridxOfs: IdxT).
-        Variables (cpRq pc cpRs' pc': IdxT).
-
-        Definition parentNumOfRules := 7.
-
-        Definition parentGetRqImm: Rule ImplOStateIfc :=
-          {| rule_idx := parentNumOfRules * ridxOfs + 0;
-             rule_msg_ids := [msiRqS];
-             rule_msgs_from := fun _ => [cpRq];
-             rule_precond :=
-               fun (ost: OState ImplOStateIfc) orq mins =>
-                 LockFree orq O /\ ost#[implStatusIdx] >= msiS;
-             rule_trs :=
-               fun (ost: OState ImplOStateIfc) orq mins =>
-                 (ost, orq,
-                  [(pc, {| msg_id := msiRsS;
-                           msg_value := VNat (ost#[implValueIdx]) |})])
-          |}.
-
-        Definition parentGetDownRqS: Rule ImplOStateIfc :=
-          {| rule_idx := parentNumOfRules * ridxOfs + 1;
-             rule_msg_ids := [msiRqS];
-             rule_msgs_from := fun _ => [cpRq];
-             rule_precond :=
-               fun (ost: OState ImplOStateIfc) orq mins =>
-                 LockFree orq O /\ ost#[implStatusIdx] = msiI;
-             rule_trs :=
-               fun (ost: OState ImplOStateIfc) orq mins =>
-                 ((hd_error mins) >>=[(ost, orq, nil)]
-                    (fun idm =>
-                       (ost,
-                        addRq orq O downRq (valOf idm) [cpRs'] pc,
-                        [(pc', {| msg_id := msiDownRqS;
-                                  msg_value := VUnit |})])))
-          |}.
-
-        Definition parentGetDownRsS: Rule ImplOStateIfc :=
-          {| rule_idx := parentNumOfRules * ridxOfs + 2;
-             rule_msg_ids := [msiDownRsS];
-             rule_msgs_from := fun _ => [cpRs'];
-             rule_precond := ⊤oprec;
-             rule_trs :=
-               fun (ost: OState ImplOStateIfc) orq mins =>
-                 ((hd_error mins) >>=[(ost, orq, nil)]
-                    (fun idm =>
-                       match msg_value (valOf idm) with
-                       | VNat n =>
-                         (ost +#[implValueIdx <- n] +#[implStatusIdx <-msiS],
-                          removeRq orq O downRq,
-                          [(pc, {| msg_id := msiRsS;
-                                   msg_value := VNat n |})])
-                       | _ => (ost, orq, nil)
-                       end))
-          |}.
-
-        Definition parentSetRqImm: Rule ImplOStateIfc :=
-          {| rule_idx := parentNumOfRules * ridxOfs + 3;
-             rule_msg_ids := [msiRqM];
-             rule_msgs_from := fun _ => [cpRq];
-             rule_precond :=
-               fun (ost: OState ImplOStateIfc) orq mins =>
-                 LockFree orq O /\ ost#[implStatusIdx] = msiM;
-             rule_trs :=
-               fun (ost: OState ImplOStateIfc) orq mins =>
-                 (ost +#[implStatusIdx <- msiI],
-                  orq,
-                  [(pc, {| msg_id := msiRsM;
-                           msg_value := VNat (ost#[implValueIdx]) |})])
-          |}.
-
-        Definition parentSetDownRqM: Rule ImplOStateIfc :=
-          {| rule_idx := parentNumOfRules * ridxOfs + 4;
-             rule_msg_ids := [msiRqM];
-             rule_msgs_from := fun _ => [cpRq];
-             rule_precond :=
-               fun (ost: OState ImplOStateIfc) orq mins =>
-                 LockFree orq O /\ ost#[implStatusIdx] <> msiM;
-             rule_trs :=
-               fun (ost: OState ImplOStateIfc) orq mins =>
-                 ((hd_error mins) >>=[(ost, orq, nil)]
-                    (fun idm =>
-                       (ost,
-                        addRq orq O downRq (valOf idm) [cpRs'] pc,
-                        [(pc', {| msg_id := msiDownRqM;
-                                  msg_value := VUnit |})])))
-          |}.
-
-        Definition parentSetDownRsM: Rule ImplOStateIfc :=
-          {| rule_idx := parentNumOfRules * ridxOfs + 5;
-             rule_msg_ids := [msiDownRsM];
-             rule_msgs_from := fun _ => [cpRs'];
-             rule_precond := ⊤oprec;
-             rule_trs :=
-               fun (ost: OState ImplOStateIfc) orq mins =>
-                 ((hd_error mins) >>=[(ost, orq, nil)]
-                    (fun idm =>
-                       match msg_value (valOf idm) with
-                       | VNat n =>
-                         (ost +#[implStatusIdx <- msiI],
-                          removeRq orq O downRq,
-                          [(pc, {| msg_id := msiRsM;
-                                   msg_value := VNat n |})])
-                       | _ => (ost, orq, nil)
-                       end))
-          |}.
-
-        Definition parentEvictRqImm: Rule ImplOStateIfc :=
-          {| rule_idx := parentNumOfRules * ridxOfs + 6;
-             rule_msg_ids := [msiRqI];
-             rule_msgs_from := fun _ => [cpRq];
-             rule_precond :=
-               fun (ost: OState ImplOStateIfc) orq mins =>
-                 LockFree orq O;               
-             rule_trs :=
-               fun (ost: OState ImplOStateIfc) orq mins =>
-                 ((hd_error mins) >>=[(ost, orq, nil)]
-                    (fun idm =>
-                       match msg_value (valOf idm) with
-                       | VNat n =>
-                         (ost +#[implValueIdx <- n] +#[implStatusIdx <- msiS],
-                          orq,
-                          [(pc, {| msg_id := msiRsI;
-                                   msg_value := VUnit |})])
-                       | _ => (ost, orq, nil)
-                       end))
-          |}.
-        
-        Definition parentRules :=
-          [parentGetRqImm; parentGetDownRqS; parentGetDownRsS;
-             parentSetRqImm; parentSetDownRqM; parentSetDownRsM;
-               parentEvictRqImm].
-
-      End Rules.
-      
-      Definition parent: Object :=
-        {| obj_idx := parentIdx;
-           obj_ifc := ImplOStateIfc;
-           obj_rules :=
-             (parentRules 0 c1pRq pc1 c2pRs pc2)
-               ++ (parentRules 1 c2pRq pc2 c1pRs pc1);
-           obj_rules_valid := ltac:(inds_valid_tac)
+      Definition parentEvictRqImm: Rule ImplOStateIfc :=
+        {| rule_idx := parentNumOfRules * ridxOfs + 6;
+           rule_msg_ids := [msiRqI];
+           rule_msgs_from := fun _ => [cpRq];
+           rule_precond :=
+             fun (ost: OState ImplOStateIfc) orq mins =>
+               LockFree orq O;               
+           rule_trs :=
+             fun (ost: OState ImplOStateIfc) orq mins =>
+               ((hd_error mins) >>=[(ost, orq, nil)]
+                 (fun idm =>
+                    match msg_value (valOf idm) with
+                    | VNat n =>
+                      (ost +#[implValueIdx <- n] +#[implStatusIdx <- msiS],
+                       orq,
+                       [(pc, {| msg_id := msiRsI;
+                                msg_value := VUnit |})])
+                    | _ => (ost, orq, nil)
+                    end))
         |}.
       
-    End Parent.
+      Definition parentRules :=
+        [parentGetRqImm; parentGetDownRqS; parentGetDownRsS;
+           parentSetRqImm; parentSetDownRqM; parentSetDownRsM;
+             parentEvictRqImm].
+
+    End Rules.
     
-    Definition impl: System :=
-      {| sys_objs :=
-           [child child1Idx ec1 ce1 c1pRq c1pRs pc1;
-              child child2Idx ec2 ce2 c2pRq c2pRs pc2;
-              parent];
-         sys_oinds_valid := ltac:(inds_valid_tac);
-         sys_minds := [c1pRq; c1pRs; pc1; c2pRq; c2pRs; pc2];
-         sys_merqs := [erq1; erq2];
-         sys_merss := [ers1; ers2];
-         sys_msg_inds_valid := ltac:(inds_valid_tac);
-         sys_oss_inits := implInit;
-         sys_orqs_inits := []
+    Definition parent: Object :=
+      {| obj_idx := parentIdx;
+         obj_ifc := ImplOStateIfc;
+         obj_rules :=
+           (parentRules 0 c1pRq pc1 c2pRs pc2)
+             ++ (parentRules 1 c2pRq pc2 c1pRs pc1);
+         obj_rules_valid := ltac:(inds_valid_tac)
       |}.
+    
+  End Parent.
+  
+  Definition impl: System :=
+    {| sys_objs :=
+         [child child1Idx ec1 ce1 c1pRq c1pRs pc1;
+            child child2Idx ec2 ce2 c2pRq c2pRs pc2;
+            parent];
+       sys_oinds_valid := ltac:(inds_valid_tac);
+       sys_minds := [c1pRq; c1pRs; pc1; c2pRq; c2pRs; pc2];
+       sys_merqs := [erq1; erq2];
+       sys_merss := [ers1; ers2];
+       sys_msg_inds_valid := ltac:(inds_valid_tac);
+       sys_oss_inits := implInit;
+       sys_orqs_inits := []
+    |}.
 
-    Definition implTopo: GTree :=
-      Node parentIdx
-           [([createEdge child1Idx c1pRq parentIdx;
-                createEdge child1Idx c1pRs parentIdx;
-                createEdge parentIdx pc1 child1Idx],
-             Node child1Idx nil);
-              ([createEdge child2Idx parentIdx c2pRq;
-                  createEdge child2Idx parentIdx c2pRs;
-                  createEdge parentIdx child2Idx pc2],
-               Node child2Idx nil)].
-                                            
-  End Impl.
-
+  Definition implTopo: GTree :=
+    Node parentIdx
+         [([createEdge child1Idx c1pRq parentIdx;
+              createEdge child1Idx c1pRs parentIdx;
+              createEdge parentIdx pc1 child1Idx],
+           Node child1Idx nil);
+            ([createEdge child2Idx parentIdx c2pRq;
+                createEdge child2Idx parentIdx c2pRs;
+                createEdge parentIdx child2Idx pc2],
+             Node child2Idx nil)].
+  
 End System.
 
 Close Scope list.
