src/Ex/Spec.v
@@ -1,0 +1,21 @@
+Require Import Bool Vector List String Peano_dec.
+Require Import Common FMap HVector ListSupport.
+
+Set Implicit Arguments.
+
+Open Scope list.
+Open Scope hvec.
+Open Scope fmap.
+
+(** Message Ids *)
+
+Definition getRq: IdxT := 0.
+Definition getRs: IdxT := 1.
+Definition setRq: IdxT := 2.
+Definition setRs: IdxT := 3.
+Definition specNumMsgIds := 4.
+
+Close Scope list.
+Close Scope hvec.
+Close Scope fmap.
+
