src/Ex/SpecSv.v
@@ -1,0 +1,126 @@
+Require Import Bool Vector List String Peano_dec.
+Require Import Common FMap HVector ListSupport Syntax Semantics StepT.
+Require Import Topology RqRs.
+
+Require Import Spec.
+
+Set Implicit Arguments.
+
+Open Scope list.
+Open Scope hvec.
+Open Scope fmap.
+
+Section System.
+  Variable numC: nat. (* if [numC = 0], then the system has a single child. *)
+
+  Definition erq (i: nat) := 2 * i.
+  Definition ers (i: nat) := 2 * i + 1.
+
+  Section Spec.
+
+    Definition specIdx := 0.
+
+    Definition SpecOStateIfc: OStateIfc :=
+      {| ost_sz := 1;
+         ost_ty := [nat:Type]%vector |}.
+    Definition specValueIdx: Fin.t 1 := Fin.F1.
+    Definition specInit: OStates :=
+      [specIdx <- {| ost_ifc := SpecOStateIfc;
+                     ost_st := hvcons 0 hvnil |}].
+    
+    Section PerChn.
+      Variable ridxOfs: nat.
+      Variables (erq ers: nat).
+
+      Definition specNumOfRules := 2.
+
+      Definition specGetRq: Rule SpecOStateIfc :=
+        {| rule_idx := specNumOfRules * ridxOfs + 0;
+           rule_msg_ids := [getRq];
+           rule_msgs_from := fun _ => [erq];
+           rule_precond := ⊤oprec;
+           rule_trs :=
+             fun (ost: OState SpecOStateIfc) orq mins =>
+               (ost, orq,
+                [(ers, {| msg_id := getRs;
+                          msg_value := VNat (ost#[specValueIdx])
+                       |})])
+        |}.
+
+      Definition specSetRq: Rule SpecOStateIfc :=
+        {| rule_idx := specNumOfRules * ridxOfs + 1;
+           rule_msg_ids := [setRq];
+           rule_msgs_from := fun _ => [erq];
+           rule_precond := ⊤oprec;
+           rule_trs :=
+             fun (ost: OState SpecOStateIfc) orq mins =>
+               ((hd_error mins) >>=[ost]
+                                (fun idm =>
+                                   match msg_value (valOf idm) with
+                                   | VNat n => ost+#[specValueIdx <- n]
+                                   | _ => ost
+                                   end),
+                orq,
+                [(ers, {| msg_id := setRs;
+                          msg_value := VUnit |})])
+        |}.
+
+    End PerChn.
+    
+    Definition specRulesI (i: nat): list (Rule SpecOStateIfc) :=
+      [specGetRq i (erq i) (ers i); specSetRq i (erq i) (ers i)].
+
+    Fixpoint specRules (i: nat): list (Rule SpecOStateIfc) :=
+      match i with
+      | O => specRulesI O
+      | S i' => (specRulesI i) ++ (specRules i')
+      end.
+
+    Lemma specObj_obj_rules_valid:
+      forall i, NoDup (map (@rule_idx _) (specRules i)).
+    Proof.
+    Admitted.
+
+    Definition specObj: Object :=
+      {| obj_idx := specIdx;
+         obj_ifc := SpecOStateIfc;
+         obj_rules := specRules numC;
+         obj_rules_valid := specObj_obj_rules_valid numC
+      |}.
+
+    Fixpoint specMerqs (i: nat): list IdxT :=
+      match i with
+      | O => [erq O]
+      | S i' => erq i :: specMerqs i'
+      end.
+
+    Fixpoint specMerss (i: nat): list IdxT :=
+      match i with
+      | O => [ers O]
+      | S i' => ers i :: specMerss i'
+      end.
+
+    Lemma spec_msg_inds_valid:
+      forall i, NoDup (nil ++ specMerqs i ++ specMerss i).
+    Proof.
+    Admitted.
+
+    Definition spec: System :=
+      {| sys_objs := [specObj];
+         sys_oinds_valid := ltac:(inds_valid_tac);
+         sys_minds := nil;
+         sys_merqs := specMerqs numC;
+         sys_merss := specMerss numC;
+         sys_msg_inds_valid := spec_msg_inds_valid numC;
+         sys_oss_inits := specInit;
+         sys_orqs_inits := []
+      |}.
+
+  End Spec.
+
+End System.
+
+Close Scope list.
+Close Scope hvec.
+Close Scope fmap.
+
